Refresh Vminus for last QC lecture and exercises

vminus/CompilerTest.v
@@ -1,4 +1,4 @@
-(** * Testing Vminus: QuickChick in the Large *)
+(** * CompilerTest: Testing Vminus: QuickChick in the Large *)
 
 Require Import List.
 Import ListNotations.
@@ -8,6 +8,7 @@ Require Import Arith.
 Require Import QuickChick.QuickChick.
 Import QcDefaultNotation. Open Scope qc_scope.
 
+Require Import Vminus.QC.
 Require Import Vminus.Classes.
 Require Import Vminus.Vminus.
 Require Import Vminus.Atom.
@@ -22,435 +23,892 @@ Require Import Vminus.AtomGen.
 Require Import Vminus.ImpGen.
 Require Import Vminus.OpSemGen.
 
+Set Warnings "-extraction-opaque-accessed,-extraction".
+Set Warnings "-extraction-logical-axiom".
+Set Warnings "-large-nat,-numbers".
 
 (* ################################################################# *)
 (** * QuickChick and Vellvm *)
-(** One may expect a compiler for a language as simple as IMP to be relatively
-    straightforward, and a proof of its correctness to be correspondingly
-    so. However, LLVM is a full-featured IR and a faithful formalization is
-    necessarily complex and large. When the compiler is under development, even
-    stating the correctness of the compiler can be difficult, much less proving
-    it.
+(** One might expect a compiler (and correctness proof) for a language
+    as simple as IMP to be relatively straightforward.
+    
+    However, LLVM -- even in its simplified Vminus form -- is a
+    somewhat complex IR, and a faithful formalization is necessarily
+    somewhat involved.  Moreover, when a compiler is under
+    development, even _stating_ its correctness can be difficult, much
+    less proving it.
 
-    But if we have interpreters for both the source and target, testing the
-    compiler is a much simpler affair. Moreover, the simplicity of the source
-    language, i.e. Imp. means that it is really easy to test! *)
+    Fortunately, _testing_ the compiler and its correctness properties
+    is a much simpler affair, as we will see. *)
 
-(** This lecture shows how QuickChick can be used to test the compiler. For
-    simplicity, the target language is the simplified SSA language Vminus, and
-    we use a variant of Imp whose names are just memory addresses which can be 
-    interpreted in the memory of Vminus states. Imp states and Vminus memory
-    are hence essentially the same, and this makes it easy to state correct 
-    compilation: after running the source program and its compilation, 
-    every Imp variable/address is mapped to the same [nat] by both the Imp 
-    state and Vminus memory. 
+(** Our target language is the simplified SSA language Vminus defined
+    in the other files in this directory, and we use a variant of Imp
+    whose names are just memory addresses which can be interpreted in
+    the memory of Vminus states. Imp states and Vminus memory are
+    hence essentially the same, and this makes it easy to state
+    correct compilation: after running the source program and its
+    compiled version, every Imp variable/address is mapped to the same
+    [nat] by both the final Imp state and the final Vminus memory. *)
 
-    A Vminus state consists of a memory (mapping addresses to [nat]), a program 
-    counter, an environment mapping locals to nat, a "previous" program 
-    counter, and a "previous" environment. The latter two are needed for
-    executing phi nodes. A configuration consists of a Vminus state and a CFG,
-    which "holds" Vminus instructions organized in basic blocks.
- *)
+(** A Vminus state consists of a memory (mapping addresses to [nat]),
+    a program counter, an environment (mapping "locals" to [nat]), a
+    "previous" program counter, and a "previous" environment; the
+    latter two are used for executing phi nodes. A configuration
+    consists of a Vminus state and a CFG, which holds Vminus
+    instructions organized in basic blocks. *)
+
+(* ################################################################# *)
+(** * Vminus Review *)
+
+(** To make this case study chapter self contained, we begin with a
+    very brief review of the relevant parts of the Vminus intermediate
+    language and compiler.  If you're already familiar with
+    Vminus (e.g., from reading the other files and working exercises),
+    you can safely skip to the next section.
+
+    A Vminus program in concrete syntax vs abstract syntax looks like
+    this (warning: program is meant to only show syntax, and is not
+    meant to make sense):
+
+
+block #1:
+ %1 = add 0 0 
+  (* binary operations can work on numeric literals, i.e. [nat] *) 
+ %2 = add %1 5 (* also, on variables *) 
+ %3 = sub %2 %1 
+ %4 = store @1 %3 
+  (* store the value held by %3 into memory at address @1 *)
+
+
+    Looking ahead a bit:
+    - The Imp store and Vminus memory are the same;
+    - Vminus addresses and Imp variables are the same (modulo the
+      [AId] constructor).
+      
+    Hence Imp programs have direct access to Vminus memory, and
+    assignment statements correspond directly to such a store
+    instruction.
+
+    Also note that %%4 is redundant here; the reason is to make the
+    abstract syntax uniform
+
+
+ %5 = store @1 1 (* We can store literals too *) 
+ %6 = load @1 
+ %7 = cbr %6 #2 #3 
+  (* conditional branch based on value held in %6, again with %7 being 
+     redundant; we can also branch on [nat] *)
+
+block #2:
+ %8 = load @1 
+ %9 = jmp #4 (* unconditional jump *)
+
+block #3:
+ %10 = load @1 
+ %11 = jmp #4
+
+block #4:
+ %12 = phi [(#2, %8) ; (#3, %10)] 
+  (* %12 takes the value held by %8 if control came from block #2, 
+     or the value held by %10 if control came from #3 *) 
+ %13 = jmp #5
+
+block #5:
+ %14 = ret (* again, variable %14 is unnecessary *)
+
+
+In the abstract syntax, every instruction is defined as:
+
+[Definition insn := (uid * cmd)%type.]
+
+In the above, the [uid] is the number on the left of the equal sign,
+and [cmd] is defined as follows:
+
+
+Inductive cmd : Set :=
+| cmd_bop : bop -> val -> val -> cmd cmd_phi : list phiarg -> cmd
+| cmd_tmn : tmn -> cmd cmd_load : addr -> cmd cmd_store : addr ->
+| val -> cmd.
+
+
+Each individual command is either a binary operation like add, a
+phi-node that joins a list of blocks, a terminator, a load, or a
+store; all of these are illustrated in the program above.
+
+Moreover, a program is represented as a control flow graph (see
+[ListCFG] for implementation and [CFG] for the interface). 
+A CFG is just a list of blocks, with one of
+them distinguished (via [lbl]) as the entry block.
+
+
+Definition t := (lbl * list block)%type. 
+Local Notation cfg := t.
+
+
+A program counter is a block label [lbl] with an offset n within the
+block.
+
+[ Definition pc := (lbl * nat)%type. ]
+
+A block has its label [lbl] and contains a list of instructions.
+
+[ Definition block := (lbl * list insn)%type. ]
+
+As the concrete syntax shows, there are 3 forms of identifiers, and
+they are all implemented as Atoms with the fresh interface.
+- [uid]: The %% prefix, e.g. %%7.
+- [addr]: The @ prefix, e.g @1.
+- [lbl]: The # prefix, e.g. #3.  A potential point of confusion would
+be that [Check], [Print], etc. shows [addr] instead of [lbl] or [uid], because
+[addr] is last-defined.
+*)
+
+(* ################################################################# *)
+(** * Overview of the Compiler *)
+
+(**
+One key part of compilation to Vminus, as an SSA form, is the need to generate
+fresh labels as we go along. Hence the compiler is implemented as a Writer 
+monad, specifically as a CMD (and EXP) following the definitions below:
+
+In [Classes.v]: 
+
+[ Definition ST (M:Type) (A:Type) := M -> (M * A).] 
+
+In [Compiler.v]:
+
+Notation EXP := (ST (list uid)).
+Definition cstate := (list lbl * list uid * list block)%type.
+Notation CMD := (ST cstate).
+
+
+The [CMD] monad is the compiler monad at the top level, handling in particular 
+control flow (that is why the block labels are threaded through). The [EXP]
+monad is for compilation within basic blocks. A subtlety: the compiler compiles 
+every Imp assignment statement to its own basic block, so basic blocks in the 
+compilation result are not maximal in the usual sense. 
+
+For both, [list uid] is the set of uids already generated thus far; similar
+interpretation for [list lbl]. The [list block] part holds the compilation 
+result thus far (recall that each block contains its own block label). 
+
+Compilation is hence activated by running the function [CMD] on appropriate
+initial (empty) lists:
+
+
+Definition compile (c:com) : ListCFG.t * lbl * lbl :=
+  let '(_, _, bs, (le, lr)) := comp_prog c ([], [], []) in
+    ((le, bs), le, lr).
+
+Definition comp_prog (c:com) : CMD (lbl * lbl) :=
+  do r <- fresh_lbl;
+  do x <- liftF fresh;
+  do _ <- add_insns r [(x, cmd_tmn tmn_ret)];
+  do e <- comp_com c r;
+  ret (e, r).
+
+
+Looking at just [compile] and the signature of [comp_prog], the compiler 
+instantiates the value part of the state monad [A] in [S * A] as [lbl * lbl].
+The first component is the entry (block) label that can be used to start 
+executing the compilation result; the second component is the label for the 
+block that control goes to -after- executing the compilation result. 
+
+Note: [le] and [lr] are used consistently to mean as such. 
+
+*)
+
+(**
+This is why the CFG (i.e. compiled program) returned has its entry label as 
+[le], and the compilation result is just [bs]. 
+
+For [comp_prog] itself: 
+- [fresh_label] creates a new block with no instructions in the compilation 
+  result, gives it a fresh label, and returns this as its value [r]
+- it generates a fresh [uid] (%%<number>) via [fresh], and returns this [x]
+- it sets, in the compilation result, the block labeled [r] to hold a 
+  return terminator instruction. To see this concretely, look at 
+  [block #5: %14 = ret] above.
+- it compiles the program [c] via [comp_com]. Note that the desired 
+  return-of-control [lbl r] is passed to it. The [lbl e] returned by [comp_com] 
+  is in turn the entry-of-control label [e].
+
+As the documentation for [comp_com] states:
+  The input [lr] is the "continuation" label of the block to which control
+  should return after the command is done.  The output is the label of the
+  entry block for the command. 
+  
+  Note how compiling a sequence [[c1;;c2]] threads the control through the 
+  commands in reverse order.
+*)
+
+
+(* ################################################################# *)
+(** * Overview of Relevant Files *)
+(**
+   - \CHAP{Vminus] defines the syntax of Vminus.
+   - [VminusOpSem] defines its semantics.   
+
+     [Inductive step (g:Cfg.t) : state -> state -> Prop] summarizes everything. 
+     A Vminus state is described below, but concretely for now:
+*)
+(**
+
+     Record state := mkst { st_mem  : mem
+                          ; st_pc   : pc
+                          ; st_loc  : loc
+                          ; st_ppc  : pc     (* predecessor pc *)
+                          ; st_ploc : loc    (* predecessor "locals" *) 
+                          }.
+*)
+(**
+   - [Compiler] shows the compiler. 
+   - [CFG] is the interface for CFGs; [ListCFG] is the implementation.
+   - [CompilerProp] holds the relevant content for what follows, and is 
+     described in-line.
+*)
 
 (* ################################################################# *)
 (** * Testing Whole-Program Compiler Correctness *)
 
-(** Here's a look at what we mean. *)
+(** Here's a property we'd like to test (from [CompilerProp]):
 
-(**
-[[Theorem compile_program_correct_terminating:
-  forall c m m' g le lr,
-  (g, le, lr) = compile c ->
-  imp_terminates c m m' ->
-  vminus_terminates g m m'.]]
+    Theorem compile_program_correct_terminating:
+      forall c m m' g le lr,
+      (g, le, lr) = compile c ->
+      imp_terminates c m m' ->
+      vminus_terminates g m m'.
 *)
 
-(** This is one of the top-level correctness theorems for the compiler: for any 
-    initial memory [m], if the source program c terminates with memory (Imp 
-    state) [m'], running the compilation result [g] (a control flow graph 
-    holding the instructions) on the same initial memory [m] also results in 
-    termination, and with its final (Vminus) memory also being [m']. This is 
-    where the coincidence of Imp states and Vminus memory comes into play.
+(** This is one of the top-level correctness theorems for the
+    compiler: for any initial memory [m], if the source program [c]
+    terminates with memory (Imp state) [m'], running the compilation
+    result [g] (a control flow graph holding the instructions) on the
+    same initial memory [m] also results in termination, and with its
+    final (Vminus) memory also being [m']. *)
+
+(** (This is where the coincidence of Imp states and Vminus
+    memory comes into play.) *)
     
-    Terminating Imp programs are those that are evaluated to just [SKIP], as the
-    following definition shows. 
- *)
 
-(** Definition imp_terminates (c: com) (m m':mem) : Prop :=
-      star Imp.step (c, m) (SKIP, m').]]
-*)
-
-(** For Vminus programs on the other hand, running them on an initial memory 
-    [m] leads to termination with memory [m'] if execution reaches a return 
-    terminator.
-*)
-
+(** Recall: An Imp program takes memory [m] to memory [m'], written
+    [imp_terminates c m m'] if, when started in [m], it multi-steps to
+    just [SKIP], with new memory [m']. *)
 (** 
-[[Definition vminus_terminates (g:ListCFG.t) (m m':mem) : Prop :=
-  exists x st',
-    insns_at_pc g st'.(st_pc) [(x, cmd_tmn tmn_ret)] /\
-    st'.(st_mem) = m' /\
-    star (step g) (init_state g m) st'.]]
+
+    Definition imp_terminates (c: com) (m m': mem) : Prop :=
+      star Imp.step (c, m) (SKIP, m').
 *)
 
-(** The variables [x] and [st'] here are determined by "running"/evaluation, as 
-    indicated by [star (step g) (init_state g m) st']. So checking for their 
-    existence is really verifying that an evaluation function reaches [st']
-    satisfying the constraints. 
+(** For Vminus programs [g], on the other hand, running on an initial
+    memory [m] leads to with memory [m'], written [vminus_terminates g
+    m m'] if execution starting from [m] reaches a return terminator
+    [tmn_ret]. *)
+(** 
+
+    Definition vminus_terminates 
+                  (g: ListCFG.t) (m m': mem) : Prop :=
+      exists x st',
+        insns_at_pc g st'.(st_pc) [(x, cmd_tmn tmn_ret)] /\
+        st'.(st_mem) = m' /\
+        star (step g) (init_state g m) st'.
 *)
 
-(** Let us try to write a Checker for the theorem. Looking at the "for all" 
-    quantifiers, it would appear that we need generators for Imp commands ([c]), 
-    Imp states/memories ([m], [m']), control flow graphs ([g]) and labels 
-    ([le], [lr]).
+(** The variables [x] and [st'] here are determined by the evaluation
+    relation, as indicated by [star (step g) (init_state g m) st']. So
+    checking for their existence can be thought of as verifying that
+    an evaluation function yields some [x] and [st'] satisfying the
+    constraints. *)
 
-    However, note that [g], [le], and [lr] are computed by [compile c], so we 
-    don't actually need generators for them. Moreover, we do not want just any 
-    [c] and [m'], but only terminating Imp programs, and [m'] is obtained by 
-    running an Imp evaluator on [m]. Hence for generation, we only need:
-    - A generator for [mem]. 
-    - A generator for Imp programs that are guaranteed to terminate. 
-    And for checking, we would need:
-    - An evaluator for Imp that reaches termination, i.e. [SKIP].
-    - An evaluator for Vminus that reaches termination, i.e. a return 
-      terminator. 
-    - We also need to check that the final state [st'] that the Vminus 
-      evaluator reaches has the desired memory.
-*)
+(** Let us try to write a [Checker] for the property
 
-(** Let us first define an evaluator for Vminus. The evaluator stops when 
-    a return terminator is reached. *)
+    Theorem compile_program_correct_terminating:
+      forall c m m' g le lr,
+      (g, le, lr) = compile c ->
+      imp_terminates c m m' ->
+      vminus_terminates g m m'.
 
-Fixpoint vminus_eval (g: ListCFG.t) (s : state) (fuel: nat) : err state :=
-  match fuel with
-  | 0 => inl "out of fuel"
-  | S n' =>
-    match (ListCFG.fetch g (st_pc s)) with
-    | Some instr =>
-      if eq_dec_cmd (snd instr) (cmd_tmn tmn_ret) then inr s
-      else
-        match (eval_step g s) with
-        | inr s' => vminus_eval g s' n'
-        | inl err => inl err
-        end
-    | None => inl "no instr to fetch"
-    end
-  end.
+    Looking naively at these "for all" quantifiers, it would appear that 
+    we need generators for Imp commands ([c]), Imp states / Vminus
+    memories ([m], [m']), control flow graphs ([g]) and labels ([le],
+    [lr]). *)
 
-(** It is likely that QuickChick will generate large enough Imp programs such 
-    that [vminus_eval] can run out of fuel. (Think of large [aexp] expressions.)
-    It is thus useful to have a generator for Imp commands whose [aexp] and 
-    [bexp] expressions are relatively small. As a first step, the following 
-    generator limits the size of [aexp] expressions to no more than 5 (where 
-    size goes by the derived generator for [aexp]).
+(** However, [g], [le], and [lr] are computed by [compile c], so we
+    don't actually need generators for them. Moreover, we do not want
+    just any [m']; rather, [m'] should be obtained by running an Imp
+    evaluator (which we have) on [m]. Hence for generation, we only
+    need
+    (1) a generator for [mem] and
+    (2) a generator for Imp programs. *)
+
+(** And for checking that the property holds, we need
+    (1) an evaluator for Vminus that repeatedly steps until it reaches a
+        return terminator and
+    (2) a way to check that the final state [st'] from the Vminus
+        evaluator has the desired memory contents. *)
+
+(** One small technical issue with all of this is that memories are
+    total maps on an infinite domain, so we cannot actually check that
+    two memories are equal.
+
+    Fortunately, for compiler testing, we only care about variables
+    that appear in the source program. So as a simplification, we fix
+    a domain of variables from which we draw when generating Imp
+    programs, and we use the same set when checking memories. *)
+
+(** The domain is fixed up front in [ImpGen] like this: *)
+
+Print id_store.
+(* ===> 
+    id_store = get_fresh_atoms 5 []
  *)
 
-(* Benjamin: Instructions not clear to me *)
-(* Nicolas: Noted with Leo's comment on giving the first as example; 
-   is the revision clearer? *)
+(** The generator [gen_id] generates fresh identifiers (atoms) by sampling from 
+    this fixed domain. *)
 
-Derive Arbitrary for aexp.
-
-Definition round_down_to (n: nat) (k: nat) :=
-  if (lt_dec n k) then n else k.
-
-Instance gen_small_aexp: GenSized aexp :=
-  {| arbitrarySized n := @arbitrarySized aexp _ (round_down_to 5 n)
-  |}.
-
-(** **** Exercise: 1 star (GenSmallBexp)  *)
-(** Write a similar GenSized instance for [bexp] that rounds down its size 
-    argument to 5. The generated instances should also have [aexp] expressions 
-    of size at most 5. *)
-
-(* FILL IN HERE *)
-(** [] *)
-
-(** For [com], recall that the lemma applies only to terminating ones. 
-    Hence, let us have two sized generators for [com]: 
-    - one that generates only assignment statements and [SKIP], such that the 
-      latter are generated with low probability.
-    - one that generates IF-THEN-ELSE, assignments and [SKIP], but no loops. 
-    The first has been done for you.
+Print gen_id.
+(* ===> 
+    gen_id = gen_fresh id_store
  *)
 
-Fixpoint gen_seq_com (n : nat) : G com :=
-  match n with 
-  | 0 => freq [(4, liftGen2 CAss arbitrary arbitrary); (1, returnGen SKIP)]
-  | S n' =>
-    let gen := gen_seq_com n' in
-    liftGen2 CSeq gen gen
-  end. 
+(** Given the generator for [id]s, we can generate [aexp], [bexp], and
+    [com] as follows. *)
 
-(** **** Exercise: 1 star (GenIfCom)  *)
-(** Write a generator for Imp [com] that generates only If-Then-Else commands, 
-    assignments, and [SKIP], but no loops. *)
+Instance gen_aexp : GenSized aexp :=
+  {
+    arbitrarySized :=
+       let base_gen := oneOf [(n <- arbitrary ;; ret (ANum n)) ;
+                              (id <- gen_id ;; ret (AId id))] in
+       fix gen_aexp_func n :=
+         match n with
+         | 0 => base_gen
+         | S n' =>
+           let binop_gen op := liftGen2 op
+                                        (gen_aexp_func n')
+                                        (gen_aexp_func n') in
+           oneOf [binop_gen APlus ;
+                  binop_gen AMinus ;
+                  binop_gen AMult;
+                  base_gen]
+         end
+  }.
 
-(* FILL IN HERE *)
-(** [] *)
+Derive Arbitrary for bexp.
+Derive Arbitrary for com.
 
-(** For your convenience, the Shows and Shrinks for [aexp], [bexp] and [com] 
-    have been defined. *)
+(** For convenience, [Show] instances for [aexp], [bexp], and [com]
+    have already been defined (in [ImpGen]). These give more
+    compact output than the ones that would automatically be
+    derived. *)
 
-(** The last thing we need a generator for is [mem]. One could generate this by 
-    first generating a subset of its domain, i.e. [Atom.t], and then generating 
-    the image for this subset; the rest would be kept as some initial value. 
-*)
+(** We also need a generator for [mem].  Given the (global) list
+    [id_store] of "interesting variables", we generate a list of
+    numeric values of the same length and use it to build a function
+    from atoms to values; other variables are set to 0. *)
 
-Definition gen_mem_from_atom_list
-           (atom_list : list Atom.t) : G mem :=
-  bindGen (vectorOf (List.length atom_list) arbitrary) (fun nat_list => 
-  returnGen (fun (a : Atom.t) =>
-               match (index_of_atom_in_list a atom_list) with
+Definition gen_mem : G mem :=
+  nat_list <- vectorOf (List.length id_store) arbitrary ;; 
+  ret (fun (a : Atom.t) =>
+               match (index_of_atom_in_list a id_store) with
                | None => 0
                | Some i =>
                  List.nth i nat_list 0
-               end)).
+               end).
 
-Check get_fresh_atoms 6 [].
-(* ===> 
-    get_fresh_atoms 6 []
-     : list addr *)
+Definition show_memory (mem: mem) : string :=
+  show_memory_on_domain mem id_store.
 
-Instance gen_domain : Gen Atom.t :=
-  {| arbitrary :=
-       let atom_store := get_fresh_atoms 100 [] in
-       oneof (returnGen (Atom.fresh [])) (List.map returnGen atom_store)
-  |}.
+(** Next let's define an evaluator for Vminus that stops when a return
+    terminator is reached (or when it gets stuck or runs out of
+    fuel -- we'll return different results in these cases so that we can
+    tell what happened later). *)
 
-(** It would be convenient to show memory too. *)
+Inductive vminus_eval_result :=
+| Terminates (st: state): vminus_eval_result
+| GoesWrong (s: string): vminus_eval_result
+| Timeout : vminus_eval_result.
 
-Check show_memory.
-(* ===> 
-    show_memory
-      : mem -> list addr -> string *)
+Fixpoint vminus_eval (g: ListCFG.t) (st : state) (fuel: nat) :
+  vminus_eval_result :=
+  match fuel with
+  | 0 => Timeout
+  | S n' =>
+    match (ListCFG.fetch g (st_pc st)) with
+    | Some instr =>
+      if eq_dec_cmd (snd instr) (cmd_tmn tmn_ret) then Terminates st
+      else
+        match eval_step g st with
+        | inr st' => vminus_eval g st' n'
+        | inl err => GoesWrong err
+        end
+    | None => GoesWrong "no instr to fetch"
+    end
+  end.
 
-(** With generation out of the way, we can now return to checking. 
-    The Vminus evaluator defined earlier solves a part of the puzzle, namely
-    the question of how to check the existence of [st'] and [x]. However, we 
-    also need to check that [st'] has the desired memory. Because memories here 
-    are total maps, we can only check for equality of memories for a specified 
-    domain. *)
+(** With generation out of the way, we can now return to checking.
+    First, a checker for equality of memories on "interesting
+    variables": *)
 
-Fixpoint memory_on_domain_checker
-         (dom: list addr) (mem1 mem2 : V.Opsem.mem) : Checker :=
+Fixpoint memory_equal_checker_on_domain
+         (dom: list addr) (mem1 mem2 : mem) : Checker :=
   match dom with
   | [] => checker true
   | (a :: l) =>
     if Nat.eqb (mem1 a) (mem2 a) then
-      memory_on_domain_checker l mem1 mem2
+      memory_equal_checker_on_domain l mem1 mem2
     else
       whenFail
         ("memory_equal: memory at " ++ (show a)
-                                    ++ " not equal:"
-                                    ++ " mem1 has " ++ (show (mem1 a))
-                                    ++ "; mem2 has " ++ (show (mem2 a))
+          ++ " not equal:" ++ " mem1 has " ++ (show_nat (mem1 a))
+                           ++ "; mem2 has " ++ (show_nat (mem2 a))
         )%string
         false
   end.
 
-(** This lets us assemble the termination checker for Vminus in full. *)
+Definition memory_equal_checker := memory_equal_checker_on_domain id_store.
 
-Definition vminus_termination_checker
-           (g: ListCFG.t) (m m': mem) (dom: list addr) : Checker :=
-  match vminus_eval g (init_state g m) 10000 with
-  | inr final_state =>
-    whenFail "vminus_termination_check: memories not equal"
-             (memory_on_domain_checker dom (st_mem final_state) m')
-  | inl err =>
-    whenFail ("vminus_termination_check: " ++ err) false
+(** Note that we define this operation to return a [Checker] rather
+    than a [bool], so that, if we find that the two memories are _not_
+    equal, we can stash away a useful error message. *)
+
+(** Now we can assemble the equal-final-state checker for Vminus. *)
+
+Axiom vminus_fuel : nat.
+Extract Constant vminus_fuel => "1000".
+
+Definition vminus_final_state_checker
+           (g: ListCFG.t) (m m': mem) : Checker :=
+  match vminus_eval g (init_state g m) vminus_fuel with
+  | Terminates final_state =>
+    whenFail "vminus_final_state_checker: memories not equal"
+             (memory_equal_checker (st_mem final_state) m')
+  | GoesWrong err => 
+      whenFail ("vminus_final_state_checker: " ++ err) false
+  | Timeout =>
+      checker tt  (* discard *)
   end.
 
-(** And therefore, the [Checker] for the lemma in full. *)
+(** And now, the [Checker] for the whole correctness property. *)
+
+Definition compile_program_correct_terminating_checker': Checker :=
+  forAllShrink arbitrary shrink (fun (c : Imp.com) =>
+  forAllShrinkShow gen_mem
+                   (fun x => []) 
+                   (fun m => show_memory m) 
+                   (fun m => 
+    let '(g, le, lr) := compile c in
+      match imp_eval c m 100 with
+      | Some s' =>
+        whenFail
+          ("cfg is: " ++ show g)
+          (vminus_final_state_checker g m s')
+      | None => checker tt (* discard the test *)
+      end)).
+
+
+(** There are a few things to note here. *)
+
+(** Firstly, note the use of [forAllShrinkShow] here, which lets us
+    choose the specific [Show] we want to use; it is needed here
+    because we don't have a [Show] instance for total maps (which are
+    essentially functions) like [mem]. *)
+
+(** Secondly, note the use of [checker tt]: This counts the test case
+    as a discard, for which we can see the count later. We could have
+    used [checker true] to treat the test as a "pass," but then we
+    might be falsely reassured if most tests succeed because they just
+    hold vacuously. *)
+
+(** And now, let's check it! *)
+
+(*! Extract Constant Test.defNumTests => "20".
+    QuickChick compile_program_correct_terminating_checker'. *)
+
+(* ===> 
+     +++ Passed 20 tests (7 discards)
+*)
+
+(** One thing to note is that we are generating non-terminating Imp
+    programs about 1/3 of the time, but the ones that are not
+    discarded all pass.
+    
+    If we start getting too many discards, one way to find out why is
+    to change [checker tt] above to fail, so that we can examine the
+    counterexamples.
+
+    But for now we can live with the discard rate. *)
+
+(** However, we also notice something else that's more problematic: Running
+    20 tests takes 15 seconds!
+
+    On reflection, this is not too surprising, as the grammar contains
+    a number of binary nodes and the [size] parameter is treated as a
+    bound on _depth_, not total number of nodes.  So our generated
+    tests are _huge_.  
+    
+    Let's see how huge... *)
+
+(** We quickly whack together some functions for calculating
+    the sizes of Imp code. *)
+
+Fixpoint size_aexp (a : aexp) :=
+  match a with
+  | ANum _ => 1
+  | AId _ => 1
+  | APlus a1 a2 
+  | AMinus a1 a2 
+  | AMult a1 a2 => size_aexp a1 + size_aexp a2 + 1
+  end.
+
+Fixpoint size_bexp (b : bexp) :=
+  match b with
+  | BTrue | BFalse => 1
+  | BEq a1 a2
+  | BLe a1 a2 => size_aexp a1 + size_aexp a2 + 1
+  | BAnd b1 b2 => size_bexp b1 + size_bexp b2 + 1
+  | BNot b => size_bexp b + 1
+  end.
+
+Fixpoint size_com (c : com) :=
+  match c with
+  | SKIP =>
+      1
+  | (x ::= a) =>
+      1 + size_aexp a
+  | (c1 ;; c2) =>
+      size_com c1 + size_com c2
+  | (IFB b THEN c1 ELSE c2 FI) =>
+      size_bexp b + size_com c1 + size_com c2
+  | (WHILE b DO c END) =>
+      size_bexp b + size_com c
+  end.
+  
+(** Now add a [collect]: *)
+
+Definition compile_program_correct_terminating_checker_collect: Checker :=
+  forAllShrink arbitrary shrink (fun (c : Imp.com) =>
+  collect (size_com c) (
+  forAllShrinkShow gen_mem
+                   (fun x => []) 
+                   (fun m => show_memory m)
+                   (fun m => 
+    let '(g, le, lr) := compile c in
+      match imp_eval c m 100 with
+      | Some s' =>
+        whenFail
+          ("cfg is: " ++ show g)
+          (vminus_final_state_checker g m s')
+      | None => checker tt 
+      end))).
+
+(** Now test: *)
+
+(*! Extract Constant Test.defNumTests => "20".
+    QuickChick compile_program_correct_terminating_checker_collect. *)
+(* ===>
+     6 : 1
+     1 : 90
+     1 : 8
+     1 : 578
+     1 : 34
+     1 : 322
+     1 : 307
+     1 : 3
+     1 : 2264
+     1 : 208
+     1 : 2
+     1 : 171
+     1 : 115
+     1 : 11
+     1 : 10
+     +++ Passed 20 tests (6 discards)
+*)
+
+(** Yep, some of these look too big *)
+
+(** To fix this, we can use the [resize] combinator to change the
+    maximum size that will be passed to sized generators to something
+    other than the default (which is 10). *)
+
+Check resize.
+(* ===> 
+        resize
+         : nat -> G ?A -> G ?A
+        where
+        ?A : [ |- Type] 
+*)
+
+(** Let's set it to 3. *)
 
 Definition compile_program_correct_terminating_checker: Checker :=
-  forAll (gen_seq_com 5) (fun (c : Imp.com) =>
-  forAll arbitrary (fun (dom : list Atom.t) => 
-  forAllShrinkShow (gen_mem_from_atom_list dom)
-                   (fun x => []) (* dummy shrinker *)
-                   (fun m => show_memory m dom) (* show just for the domain *)
+  forAllShrink (resize 3 arbitrary) shrink (fun (c : Imp.com) =>
+  forAllShrinkShow gen_mem
+                   (fun x => []) 
+                   (fun m => show_memory m) 
                    (fun m => 
-  let '(g, le, lr) := compile c in
-    match imp_eval c m 100 with
-    | Some s' =>
-      vminus_termination_checker g m s' dom
-    | None => whenFail "compile_program_termination: cannot eval imp to Skip"
-                      false
-    end))).
+    let '(g, le, lr) := compile c in
+      match imp_eval c m 100 with
+      | Some s' =>
+        whenFail
+          ("cfg is: " ++ show g)
+          (vminus_final_state_checker g m s')
+      | None => checker tt (* discard the test *)
+      end)).
 
-(** Note the use of [forAllShrinkShow] here, which lets us choose the specific 
-    Show we want to use; it is needed here because we don't have a [Show] 
-    instance for total maps (which are essentially functions) like [mem]. *)
+(** Now we can run 10000 tests in a few seconds: *)
 
-(* ! QuickChick compile_program_correct_terminating_checker. *)
+(*! QuickChick compile_program_correct_terminating_checkers. *)
+(* ===>
+    +++ Passed 10000 tests (2841 discards)
+*)
+
+(** EX2 (GenComWithSmallExpr) *)
+(** Add a [collect] to the checker that collects the exact Imp command
+    for each test.  Set [defNumTests] to 20 to avoid looking at too
+    many examples, and use QuickChick to take a look.  Notice that the
+    generated programs tend to be quite short but that they tend to
+    involve quite large arithmetic and/or boolean expressions.  This
+    distribution may not be giving us the most effective testing.
+
+    Write a generator for [com] that takes a size bound [n] and
+    generates commands in which [bexp] and [aexp] expressions have
+    size at most [n]. *)
+(* FILL IN HERE *)
+(** [] *)
+
+(** EX1 (IdentifyDiscards) *)
+(** By design of the Checker, we expect discards to be due to non-terminating 
+    programs. To investigate this, change the Checker so that "out of fuel" 
+    is treated as a failure. Is the counterexample what you expect? Can you 
+    be absolutely sure that such counterexamples are due to "out of fuel" 
+    rather than because of a genuine bug? *)
+
+(* FILL IN HERE *)
+(** [] *)
+
+(* ################################################################# *)
+(** * Mutation Testing *)
+
+(** Beyond discarded tests, we are also interested in the tests that
+    _pass_.  In particular, we want to make sure that they are passing
+    because the property really holds, rather than some oversight in
+    generation or formulation of the Checker. To do that, we can
+    _mutate_ the compiler to falsify the property and check that the
+    Checker fails in this case.
+
+    _Mutation testing_ is a powerful technique for increasing
+    confidence in the quality of our tests.  QuickChick comes with a
+    command-line tool for mutation testing, but it isn't quite able
+    yet to handle the Vminus development.  So for the moment we'll
+    just play with mutants manually. *)
+
+(** We've left a suggested mutant in a comment in the [APlus] case of the
+    [comp_aexp] function in [Compiler].
+    
+    Inserting this mutant gives us the following. *)
+
+(*! QuickChick compile_program_correct_terminating_checker. *)
+(** ===> 
+
+    QuickChecking compile_program_correct_terminating_checker
+    Id 4 := (ANum 60 + ANum 25)
+    mem: [(addr 5, 77) (addr 4, 73) (addr 3, 34) 
+          (addr 2, 21) (addr 1, 59) ]
+    cfg is: (entry 2, blks: lbl 1: []
+    vminus_final_state_checker: memories not equal
+    memory_equal: memory at Id 4 not equal: mem1 has 35; mem2 has 85
+    *** Failed after 67 tests and 31 shrinks. (40 discards)
+*)
+
+(** **** Exercise: 2 stars (comp_aexp_minus_mutant)  *)
+(** Do the same for the suggested mutant for the [AMinus] case in [comp_aexp].
+    Repeat the experiment for a few times. Are the results what you expect? 
+    Investigate why. *)
+
+(*! QuickChick compile_program_correct_terminating_checker. *)
+
+(* FILL IN HERE *)
+(** [] *)
+
+(** This finishes the testing of the top-level compiler correctness
+    property.
+
+    Compare the relative ease of developing this testing
+    infrastructure with what's involved in proving the theorem!
+
+    The key part of that proof involves defining a [match_states]
+    relation very carefully, and it can take many iterations to get it
+    right, both in terms of correctness and sufficiency for the proof
+    to go through.  This is on top of making sure that the compiler
+    has no bugs.
+ 
+    Testing can help us to quickly pin down bugs in the compiler
+    itself, so that we can focus on the proof.  In contrast to the
+    proof development, our generators have all been automatically
+    derived, and writing the Checker for this is considerably
+    simpler. *)
 
 (* ################################################################# *)
 (** * Testing Lemmas for Compiler Correctness *)
 
-(** For the next part, consider the sort of lemmas that would be needed 
-    to prove the top-level correctness theorems like the one above. Here's one.
-*)
+(** Next, let's look at a property for which the infrastructure needed
+    for testing is a bit more elaborate: one of the lemmas that is
+    used in proving the top-level correctness theorem... *)
 
 (**
-[[Lemma comp_aexp_correct : forall (a:aexp),
-    comp_correct (comp_aexp a) (aeval a).]]
 
-[[Definition comp_correct (comp : FRESH (val * list insn))
-           (eval : mem -> nat) : Prop :=
-  forall (cs cs': list uid) (g: ListCFG.t) (st: V.Opsem.state)
-    (is k: list insn) (v: val), 
-    (cs', (v, is)) = comp cs ->
-    insns_at_pc g (st_pc st) (is ++ k) ->
-    exists st',
-      st_mem st' = st_mem st /\
-      insns_at_pc g (st_pc st') k /\
-      star (step g) st st' /\
-      ids_preserved cs st st' /\
-      good_return cs' v /\
-      ctx_incr cs cs' /\
-      eval_val (st_loc st') v = Some (eval (st_mem st)).]]
+    Lemma comp_aexp_correct : forall (a:aexp),
+        comp_correct (comp_aexp a) (aeval a).
+
+where [comp_correct] is Vminus's generic "expression compilation correctness" 
+property (used for both arithmetic and boolean expressions)... *)
+(**
+
+    Definition comp_correct (comp : FRESH (val * list insn))
+               (eval : mem -> nat) : Prop :=
+      forall (cs cs': list uid) (g: ListCFG.t) (st: V.Opsem.state)
+             (is k: list insn) (v: val), 
+   
+        (cs', (v, is)) = comp cs ->
+        insns_at_pc g (st_pc st) (is ++ k) ->
+
+        exists st',
+          (* interesting part: *)
+          st_mem st' = st_mem st /\
+          insns_at_pc g (st_pc st') k /\
+          star (step g) st st' /\ 
+          eval_val (st_loc st') v = Some (eval (st_mem st)) /\
+
+          (* details: *)
+          ids_preserved cs st st' /\
+          good_return cs' v /\
+          ctx_incr cs cs'.
 *)
 
-(** That is, compiling Imp aexp is correct if:
-    - for any compilation run on an initial list of [uid]s, 
-    - wherever we place the compilation result [is] in the CFG, as long
-      as the program counter is pointed to it
-      ([insns_at_pc g (st_pc) (is ++ k)]),
-    - we can run to the end of compilation ([insns_at_pc g (st_pc st') k]),
-    - and in this state [st'], the memory is the same as above; but evaluating 
-      the result of the expression in this state ([eval_val (st_loc st') v])
-      is exactly the same as evaluating it according to the Imp state
-      ([eval (st_mem st)]).
-    - This last fact may not be obvious from the body of [comp_correct]. But 
-      note [comp_aexp_correct]; the evaluation function passed to it is Imp's 
-      [aeval], and this is where the coincidence of Imp states and Vminus 
-      memory comes into play.
-    There is a bunch of other things that we need here, so as to prove correct
-    compilation for com. But the above description is the crux. *)
+(** That is, compiling Imp [aexp] is correct if:
+        - for _any compilation_ of some expression run on an initial
+          list of [uid]s,
+        - wherever we place the compilation _result_ [is] in the
+          _CFG_, with the program counter pointing to it ([insns_at_pc
+          g (st_pc) (is ++ k)]),
+        - _we can run to the end_ of the compiled code and reach a
+          state [st'] ([insns_at_pc g (st_pc st') k]), and
+        - in this state [st'], the _memory is the same_ as
+          above ([st_mem st' = st_mem st]), and
+        - _evaluating the result_ of the expression in this
+          state ([eval_val (st_loc st') v]) is _exactly the same_ as
+          evaluating it according to the Imp state ([eval (st_mem
+          st)]).
+    
+    This last fact may not be obvious from the body of
+    [comp_correct]. But note [comp_aexp_correct], which passes Imp's
+    [aeval] as the evaluation function.  (This is where the
+    coincidence of Imp states and Vminus memory comes into play.)
 
-(** Looking at [comp_correct], it is clear that we need to generate more than 
-    just the things we had before. In particular, it would seem that we need 
-    generators for the following:
-    - [uid]
-    - CFG ([ListCFG.t])
-    - Vminus states
-    - Vminus instructions
-    - values ([val])
-    But note again that the only value [v] is computed by comp 
-    rather than generated, so we don't actually need a generator for [val]. 
-    Moreover, the CFG [g] should not be generated randomly the same way we do 
-    others, because it has to satisfy [insns_at_pc]; it is unlikely for just 
-    "any" CFG to satisfy this precondition of the lemma. *)
+    There are a few other details that are needed for proving correct
+    compilation for [com].  But the above is the crux. *)
 
-(** **** Exercise: 1 star (GenUidInsn)  *)
-(** Have Generators and Shows for [uid] and Vminus [insn], using 
-    automation as much as possible. (It is however useful to have custom 
-    Shows that are more descriptive.) *)
+(** Looking at [comp_correct], it is clear that we need to generate
+    more than just the things we had before. In particular, it would
+    seem at first that we need several new generators:
+      - [uid]
+      - CFG ([ListCFG.t])
+      - Vminus states
+      - values ([val])
 
-(* @Benjamin: All generators and shows required for this have already been
-   defined in VminusGen.v, and this is already imported; so the lecture can 
-   continue uninterrupted with no definitions for these at this point. *)
+    But note that the only value here, [v], is computed by [comp], so
+    we don't actually need a generator for [val].  Moreover, the CFG
+    [g] _cannot_ be generated randomly, since it has to satisfy
+    [insns_at_pc] -- something that a random CFG is very unlikely to
+    do. *)
 
-(** For Vminus states, we already have a generator for [mem]. We have defined a 
-    generator and show for [loc] for you. *)
+(** **** Exercise: 2 stars (GenUidInsn)  *)
+(** Derive generators and write [Show] instances for [uid] and Vminus [insn].
+    Note that it is useful to have custom [Show] instances that are more 
+    descriptive than the default ones. *)
+(** [] *)
 
-Check gen_loc_from_atom_list.
+(** For Vminus states, we already have a generator for the [mem]
+    component.  A generator and Show for [loc] are defined in
+    [OpSemGen], with the following types: *)
+
+Check gen_loc.
 (* ===> 
-    gen_loc_from_atom_list
-     : list uid -> G loc *)
+    gen_loc
+     : G loc *)
 
 Check show_locals.
 (* ===> 
     show_locals
      : loc -> list uid -> string *)
 
-(** We can then define a generator and a show function for Vminus states, 
-    given domains for [mem] and [loc]. For simplicity, we use the same 
-    domain for [ploc]. 
- *)
+(** We can then define a generator and a [show] function for Vminus
+    states, on the fixed domains for [mem] and [loc]. *)
 
-Definition gen_vminus_state
-           (mem_dom: list Atom.t)
-           (loc_dom: list Atom.t) : G state :=
-       let gmem := gen_mem_from_atom_list mem_dom in
-       let gloc := gen_loc_from_atom_list mem_dom in
-       bindGen gmem (fun mem =>
-       bindGen arbitrary (fun pc =>
-       bindGen gloc (fun loc =>
-       bindGen arbitrary (fun ppc =>
-       bindGen gloc (fun prev_loc =>
-         returnGen
-           (mkst mem
-                 pc
-                 loc
-                 ppc
-                 prev_loc)))))).
+Definition gen_vminus_state : G state :=
+  mem <- gen_mem ;;
+  pc <- arbitrary ;;
+  loc <- gen_loc ;;
+  ppc <- arbitrary ;;
+  prev_loc <- gen_loc ;;
+  ret (mkst mem pc loc ppc prev_loc).
 
-Definition show_vminus_state
-           (mem_dom: list Atom.t)
-           (loc_dom: list Atom.t)
-           (st: state) : string :=
-  (show_memory (st_mem st) mem_dom ++ ", " ++
-               "pc: " ++ show (st_pc st) ++ ", " ++
-               show_locals (st_loc st) loc_dom ++ ", " ++
-               "ppc: " ++ show (st_ppc st) ++ ", " ++
-               "prev_loc: " ++ show_locals (st_ploc st) loc_dom)%string.
+Definition show_vminus_state (st: state) : string :=
+  (show_memory (st_mem st) ++ ", " ++
+   "pc: " ++ show (st_pc st) ++ ", " ++
+   show_locals (st_loc st) ++ ", " ++
+   "ppc: " ++ show (st_ppc st) ++ ", " ++
+   "prev_loc: " ++ show_locals (st_ploc st))%string.
 
-(** With these out of the way, we can now address the remaining gaps. In its 
-    current form, [comp_correct] is inefficient and challenging for testing. 
-    Firstly, some of the quantities are computed by a function, so it is 
-    unnecessary to generate them in the first place, although seemingly 
-    suggested by "forall". Secondly, the CFG [g] is not just any CFG, but one 
-    that satisfies [insns_at_pc] for the compilation result - random generation 
-    in the usual way is very, very unlikely to meet this condition, so most
-    checks would end up being vacuously true. Thirdly, a [Checker] for the 
-    the existence of [st'] really needs to compute it, and this is not part of
-    the lemma itself. 
+(** One deficiency of this function is that it only shows [mem] and 
+    [loc] on their respective fixed domains. You may find it more useful 
+    to have a general one that takes respective domains as input. *) 
 
-    Hence the first order of affairs is to massage the lemma into a 
-    [Checker]-friendly version.
- *)
+(** With these out of the way, we can address the remaining gaps.
+       - Firstly, some of the quantities are computed by a function,
+         so it is unnecessary to generate them.
+       - Secondly, the CFG [g] cannot be just _any_ CFG, but one that
+         satisfies [insns_at_pc] for the compilation result.  (Random
+         generation in the usual way is extremely unlikely to meet
+         this condition, so most checks would end up being vacuously
+         true.)
+       - Thirdly, a [Checker] for the existence of [st'] really
+         needs to compute it.
+*)
 
-(** Firstly, let us drop the unnecessary variables, and note the generation 
-    of [state].
+(** Firstly, let us drop the unnecessary quantified variables.
 
     Definition comp_correct (comp : FRESH (val * list insn))
                             (eval : mem -> nat) : Prop :=
       forall (cs: list uid) (g: ListCFG.t) (k: list insn),
-      forall (mem_dom: list Atom.t) (loc_dom: list Atom.t) (st: state),
+      forall (st: state),
 
       let (cs', (v, is)) := comp cs in
-
       insns_at_pc g (st_pc st) (is ++ k) ->
+
       exists st',
         st_mem st' = st_mem st /\
         insns_at_pc g (st_pc st') k /\
-        star (Opsem.step g) st st' /\
+        star (Opsem.step g) st st' /\ 
+        eval_val (st_loc st') v = Some (eval (st_mem st)) /\
+
         ids_preserved cs st st' /\
         good_return cs' v /\
-        ctx_incr cs cs' /\
-        eval_val (st_loc st') v = Some (eval (st_mem st)).
+        ctx_incr cs cs'.
 
-    This is of course not accepted by Coq, but we will eventually get to a
-    [Checker].
- *)
+    (This is, of course, not accepted by Coq yet.) *)
 
-(** Secondly, we need to write a custom generator that generates CFGs 
-    satisfying [insns_at_pc]. An easier option is to just construct a CFG that 
-    loads the instructions at a given pc. 
+(** Secondly, we need to write a custom generator that generates CFGs
+    satisfying [insns_at_pc]. An easy option is to just construct a
+    CFG that places the instructions at a given pc.
 
-    Let us call this [wrap_code_in_cfg' pc is k], in correspondence with 
-    [insns_at_pc g (st_pc st) (is ++ k)].
+    Let us call this [wrap_code_in_cfg' pc is k], in accordance with
+    [insns_at_pc g (st_pc st) (is ++ k)].  It returns a CFG with a
+    single block containing [is ++ k] placed at (position) [pc]. *)
 
-    However, because [pc] may have a positive offset into the block, we should 
-    also fill the initial instructions with some dummy instructions (that won't
-    be executed). So we make [wrap_code_in_cfg'] do this. 
-*)
-
-(* Returns a CFG with a single block containing [instrs ++ instrs_after], 
-    and the pc in that block that begins at [instrs_after] *)
-Definition wrap_code_in_cfg' (p: pc) (instrs instrs_after: list insn)
-  : ListCFG.t :=
+Definition wrap_code_in_cfg'
+              (p: pc) (instrs instrs_after: list insn)
+         : ListCFG.t :=
   let empty_cfg := [] in
   let '(lbl, offset) := p in
   let blocks :=
@@ -459,100 +917,112 @@ Definition wrap_code_in_cfg' (p: pc) (instrs instrs_after: list insn)
                         ++ instrs ++ instrs_after) in
   (lbl, blocks).
 
-(** The to-be-Checkable lemma is thus:
+(** One fine point is that, because [pc] may have a positive offset
+    into the block, we also need [wrap_code_in_cfg'] to fill the
+    initial instructions with some dummy instructions (that won't be
+    executed). *)
 
-    [[Definition comp_correct (comp : FRESH (val * list insn))
+(** Our checkable-lemma-in-progress now looks like this:
+
+    Definition comp_correct (comp : FRESH (val * list insn))
                             (eval : mem -> nat) : Prop :=
-      forall (cs: list uid) (k: list insn),
-      forall (mem_dom: list Atom.t) (loc_dom: list Atom.t) (st: state),
+      forall (cs: list uid) (k: list insn), forall (st: state),
 
       let (cs', (v, is)) := comp cs in
-      let g := wrap_code_in_cfg (st_pc st) is k in
+      let g := wrap_code_in_cfg' (st_pc st) is k in
 
       exists st',
         st_mem st' = st_mem st /\
         insns_at_pc g (st_pc st') k /\
         star (Opsem.step g) st st' /\
+        eval_val (st_loc st') v = Some (eval (st_mem st)) /\
+
         ids_preserved cs st st' /\
         good_return cs' v /\
-        ctx_incr cs cs' /\
-        eval_val (st_loc st') v = Some (eval (st_mem st)).]]
+        ctx_incr cs cs'.
 *)
 
-(** Thirdly, we know that [st'] is given by executing the compilation result; 
-    this is the point of "loading" the compilation result at the current [pc] 
-    in [g], and is of course also stated by [star (Opsem.step g) st st']. So we 
-    need an executable evaluator for Vminus. The state [st'] is obtained by 
-    running this evaluator until we reach (the start of) [k].
+(** Thirdly, we know that [st'] is given by executing the compilation
+    result; this is the point of "loading" the compilation result at
+    the current [pc] in [g], and is of course also stated by
+    [star (Opsem.step g) st st']. So we need an executable evaluator
+    for Vminus. The state [st'] is obtained by running this evaluator
+    until we reach (the start of) [k].
     
-    The simplest way of doing so is to stop at the program counter that begins
-    [k], and this is actually determined by the CFG that loaded [is ++ k]. 
+    The simplest way of doing so is to stop at the program counter
+    that begins [k], and this is actually determined by the CFG that
+    loaded [is ++ k].
 
-    Hence we change [wrap_code_in_cfg] to return [(g, pc)], where the latter is 
-    the [pc] that begins [k]. *)
+    Hence we change [wrap_code_in_cfg'] to return [(g, pc)], where the
+    latter is the [pc] that begins [k]... *)
 
 Definition wrap_code_in_cfg (p: pc) (instrs instrs_after: list insn)
   : ListCFG.t * pc :=
   let empty_cfg := [] in
   let '(lbl, offset) := p in
   let blocks :=
-      ListCFG.update empty_cfg lbl
-                     ((generate_dummy_insns offset)
-                        ++ instrs ++ instrs_after) in
+      ListCFG.update
+        empty_cfg lbl
+        ((generate_dummy_insns offset)
+         ++ instrs ++ instrs_after) in
   ((lbl, blocks), (lbl, offset + List.length instrs)).
 
-(** Now we need the evaluator itself, which we have defined for you. *)
+(** Next we need the evaluator itself (the definitions are in
+    [VminusOpSem]). *)
 
-Check V.Opsem.eval_until_pc.
+Check eval_until_pc.
 (* ===> 
     eval_until_pc
       : ListCFG.t -> state -> pc -> nat -> err state *)
 
-Check V.Opsem.eval_step.
+Check eval_step.
 (* ===>
     eval_step
      : ListCFG.t -> state -> err state *)
 
 (** Now the lemma is:
 
-    [[Definition comp_correct (comp : FRESH (val * list insn))
+    Definition comp_correct (comp : FRESH (val * list insn))
                             (eval : mem -> nat) : Prop :=
       forall (cs: list uid) (k: list insn),
-      forall (mem_dom: list Atom.t) (loc_dom: list Atom.t) (st: state),
+      forall (st: state),
 
       let (cs', (v, is)) := comp cs in
       let (g, endpoint) := wrap_code_in_cfg (st_pc st) is k in
 
-      match V.Opsem.eval_until_pc g st cutpoint 1000 with
+      match eval_until_pc g st cutpoint 1000 with
       | inl err => false (* either out of fuel or no st' *)
       | inr st' => 
-        st_mem st' = st_mem st /\
-        insns_at_pc g (st_pc st') k /\
-        star (Opsem.step g) st st' /\
-        ids_preserved cs st st' /\
-        good_return cs' v /\
-        ctx_incr cs cs' /\
-        eval_val (st_loc st') v = Some (eval (st_mem st))
-      end.]]
- *)
-
-(** And with this, the major obstacles are out of the way, and we only have
-    to write a [Checker] for the big conjunction. Because the conjunction is 
-    huge, it is easier to write a [Checker] for each conjunct. That is, we would
-    like to have:
-    - A [Checker] that checks that two memories are the same. This has already 
-      been done.
-    - A [Checker] that checks for [insns_at_pc].
-    - A [Checker] for [ids_preserved].
-    - A [Checker] for [good_return].
-    - A [Checker] for [ctxt_incr].
-    - A [Checker] that checks for equality between the two ways of evaluation.
-    Note that [star (Opsem.step g) st st'] doesn't need checking, because it is
-    implicit in [eval_until_pc]. With respect to correctness of [aexp] 
-    compilation itself, the last is most relevant. 
-
-    These are defined below.
+          st_mem st' = st_mem st /\
+          insns_at_pc g (st_pc st') k /\
+          star (Opsem.step g) st st' /\
+          eval_val (st_loc st') v = Some (eval (st_mem st)) /\
+          ids_preserved cs st st' /\
+          good_return cs' v /\
+          ctx_incr cs cs' 
+      end.
 *)
+
+(** At this point, the major obstacles are out of the way; we just
+    have to write a [Checker] for the big conjunction. Because it is
+    big, it is easier to write a [Checker] for each conjunct rather
+    than one monolithic checker.
+
+    That is, we need to define:
+      - A [Checker] that checks that two memories are the same. This
+        has already been done.
+      - A [Checker] that checks for [insns_at_pc].
+      - A [Checker] for [ids_preserved].
+      - A [Checker] for [good_return].
+      - A [Checker] for [ctxt_incr].
+      - A [Checker] that checks for equality between the two results
+        of evaluation. *)
+
+(** (Note that [star (Opsem.step g) st st'] doesn't need
+    checking, because it is implicit in [eval_until_pc].) *)
+
+(** The remaining ones are defined below.  All are fairly
+    straightforward. *)
 
 Fixpoint loc_on_domain_checker
          (dom: list uid) (loc1 loc2 : loc) : Checker :=
@@ -585,21 +1055,9 @@ Fixpoint insns_at_pc_checker `{Show pc}
     end
   end.
 
-Definition eval_equal_checker (eval: mem -> nat) (st: state) (v: val)
-  : Checker :=
-  let run_result := eval_val (st_loc st) v in
-  let expected_result := eval (st_mem st) in
-  match run_result with
-  | Some n =>
-    whenFail "eval_equal: evaluation value not the same"
-             (Nat.eqb n expected_result)
-  | None => whenFail "eval_equal: run did not obtain any value" false
-  end.
-
 Definition ids_preserved_checker (cs : list uid) (st st': state)
   : Checker :=
   loc_on_domain_checker cs (st_loc st) (st_loc st').
-
 
 Definition good_return_checker (cs: list uid) (v: val) : Checker :=
   match v with
@@ -620,99 +1078,135 @@ Fixpoint ctx_incr_checker (cs cs': list uid) : Checker :=
     else whenFail ("ctx_incr: " ++ show uid ++ " not found") false
   end.
 
-(** We can now compose the checkers using QuickChick's [conjoin] combinator. *)
+Definition eval_equal_checker (eval: mem -> nat) (st: state) (v: val)
+  : Checker :=
+  let run_result := eval_val (st_loc st) v in
+  let expected_result := eval (st_mem st) in
+  match run_result with
+  | Some n =>
+    whenFail "eval_equal: evaluation value not the same"
+             (Nat.eqb n expected_result)
+  | None => whenFail "eval_equal: run did not obtain any value" false
+  end.
+
+(** We can now compose all these checkers using QuickChick's [conjoin]
+    combinator. *)
+
 Definition expression_step_checker
-           (eval: V.Opsem.mem -> nat)
+           (eval: mem -> nat)
            (g: ListCFG.t)
-           (initial_state final_state: V.Opsem.state)
+           (initial_state final_state: state)
            (k: list insn) (end_of_expr: pc)
            (cs cs': list uid)
            (v : val) : Checker :=
-  conjoin [ids_preserved_checker cs initial_state final_state;
-             insns_at_pc_checker g end_of_expr k;
-             good_return_checker cs' v;
-             ctx_incr_checker cs cs';
-             eval_equal_checker eval final_state v].
+  conjoin [
+      ids_preserved_checker cs initial_state final_state;
+      insns_at_pc_checker g end_of_expr k;
+      good_return_checker cs' v;
+      ctx_incr_checker cs cs';
+      eval_equal_checker eval final_state v
+    ].
 
-(** Finally, a Checker for [comp_correct] and [comp_aexp] could look like the 
-    following. It is convenient to split the [Checker] into a part that does 
-    only the generation, and a part that does the checking, because a type 
-    error can cause the typechecker to get stuck trying to resolve the issue
-    by looking for typeclass instances that don't exist.    
-*)
+(** At last, we can assemble a checker for [comp_correct] as follows. *)
+
+(** (It is convenient to split the [Checker] into a part that does
+    only the generation and a second part that does the checking,
+    because a type error can cause the typechecker to get stuck trying
+    to resolve the issue by looking for typeclass instances that don't
+    exist.) *)
 
 Definition comp_correct_checker_inner
-           (comp: FRESH (val * list insn)) (eval: V.Opsem.mem -> nat)
-           (cs : list uid) (st: V.Opsem.state) (k: list insn)
-  : Checker :=
+             (comp: FRESH (val * list insn)) (eval: mem -> nat)
+             (cs : list uid) (st: state) (k: list insn)
+         : Checker :=
   let '(cs', (v, instrs)) := comp cs in
-  let '(g, endpoint) := wrap_code_in_cfg (V.Opsem.st_pc st) instrs k in
-  match V.Opsem.eval_until_pc g st endpoint 1000 with
+  let '(g, endpoint) := wrap_code_in_cfg (st_pc st) instrs k in
+  match eval_until_pc g st endpoint 1000 with
   | inl err => whenFail ("comp_correct_checker: " ++ err) false
   | inr st' => 
     expression_step_checker eval g st st' k endpoint cs cs' v
   end.
 
 Definition comp_correct_checker
-           (comp: FRESH (val * list insn)) (eval: V.Opsem.mem -> nat)
-  : Checker :=
+             (comp: FRESH (val * list insn)) (eval: mem -> nat)
+         : Checker :=
   forAll arbitrary (fun (cs : list uid) =>
   forAll arbitrary (fun (extra_insn : list insn) =>
-  forAll arbitrary (fun (mem_dom: list Atom.t) =>
-  forAll arbitrary (fun (loc_dom: list Atom.t) =>
-  forAllShrinkShow (gen_vminus_state mem_dom loc_dom)
+  forAllShrinkShow gen_vminus_state
                    (fun x => [])
-                   (show_vminus_state mem_dom loc_dom)
+                   show_vminus_state
                    (fun (start_state: state) => 
     comp_correct_checker_inner
       comp eval
-      cs start_state extra_insn))))).
+      cs start_state extra_insn))).
 
-(**! Section test_compile_aexp extends compiler *)
+(** The [comp_aexp] checker is now just a simple wrapper. *)
+
 
 Definition comp_aexp_correct_checker :=
-  forAll arbitrary (fun a: aexp =>
+  forAllShrink (resize 3 arbitrary) shrink (fun a: aexp =>
     comp_correct_checker (comp_aexp a) (aeval a)).
 
-(* ! QuickChick comp_aexp_correct_checker. *)
+(*! QuickChick comp_aexp_correct_checker. *)
+(* ===> 
+    QuickChecking comp_aexp_correct_checker
+    +++ Passed 10000 tests (0 discards)
+*)
 
-(** Since the compiler has already been proven correct, all tests should 
-    succeed. However, they could be succeeding for rather vacuous reasons, and 
-    it would be assuring to know that the [Checker] indeed fails when the 
-    compiler is wrong. 
+(** **** Exercise: 2 stars (add_aexp_mutants)  *)
+(** Since the compiler has already been proven correct, we'd expect
+    the above test to succeed. However, it could be succeeding for
+    silly reasons (because our test-case generation is bad or the
+    distribution of tests is skewed in some way), so we'd also like to
+    know that the [Checker] indeed fails when the compiler is wrong.
 
-    Exercise: Add mutants to [comp_aexp], and verify that they are causing 
-    [comp_aexp_correct_checker] to fail. 
- *)
+    Change the definition of [compile_aexp] in [Compiler] to
+    misbehave in some way (two suggestions can be found in a comment
+    there), recompile that file, then come back here and check that
+    the QuickChick command above can find the bug. *)
 
-(* END OF LECTURE *)
-
-(** **** Exercise: 1 star (compBopCorrect)  *)
-(** Write a Checker for [comp_bop_correct] in [CompilerProp.v], and make sure
-    that all tests pass.
- *)
+(** **** Exercise: 2 stars (compBopCorrect)  *)
+(** Write a Checker for [comp_bop_correct] in [CompilerProp.v], and
+    make sure that all tests pass. Next, mutate [comp_bop] in
+    [Compiler.v] to do something wrong (a suggestion is provided, but
+    again you can make up your own as well), and use QuickChick to
+    test the Checker again. Do you get a nice-looking counterexample,
+    and can you explain why it fails? *)
 
 (* FILL IN HERE *)
 (** [] *)
 
-(** **** Exercise: 1 star (compBexpCorrect)  *)
-(** Write a Checker for [comp_bexp_correct] in [CompilerProp.v], and make sure 
-    that all tests pass. 
-*)
+(** **** Exercise: 2 stars (compBexpCorrect)  *)
+(** Write a Checker for [comp_bexp_correct] in [CompilerProp.v], and
+    make sure that all tests pass. Next, mutate [comp_bexp] in
+    [Compiler.v] to do something wrong, and QuickChick your checker
+    again. Do you get a useful counterexammple? *)
 
 (* FILL IN HERE *)
 (** [] *)
 
 (** **** Exercise: 3 stars (compStoreCorrect)  *)
-(** Write a Checker for [comp_store_correct] in [CompilerProp.v], and make sure 
-    that all tests pass. *)
+(** Write a Checker for [comp_store_correct] in [CompilerProp.v], and
+    make sure that all tests pass. Next, mutate [comp_store] in
+    [Compiler.v] to do something wrong and QuickChick your Checker
+    again.  Are you happy? *)
 
 (* FILL IN HERE *)
 (** [] *)
 
-(** **** Exercise: 2 stars (compCondCorrect)  *)
-(** Write a Checker for [comp_cond_correct] in [CompilerProp.v], and make sure 
-    that all tests pass. *)
+(** **** Exercise: 3 stars (compCondCorrect)  *)
+(** Write a Checker for [comp_cond_correct] in [CompilerProp.v], and
+    make sure that all tests pass. Next, mutate [comp_cond] in
+    [Compiler.v] to do something wrong and QuickChick your checker
+    again. *)
 
 (* FILL IN HERE *)
 (** [] *)
+
+(** **** Exercise: 5 stars (check_type_safety)  *)
+(* Build checkers corresponding to the [progress] and [preservation]
+   properties in [VminusStatics].  Mutate some of the definitions
+   to introduce bugs and see if you can find them. *)
+(* FILL IN HERE *)
+(** [] *)
+
