vminus/ImpGen.v
@@ -11,6 +11,7 @@ Require Import String.
 Require Import QuickChick.QuickChick.
 Import QcDefaultNotation. Open Scope qc_scope.
 
+Require Import Vminus.QC.
 Require Import Vminus.Atom.
 Require Import Vminus.Imp.
 
@@ -21,17 +22,13 @@ Generalizable All Variables.
 (** ** id **)
 Definition id_store := get_fresh_atoms 5 [].
 
-Instance gen_id: Gen id :=
-  {| arbitrary := gen_fresh id_store |}.
-
-Instance gen_ids: GenSized (list id) :=
-  {| arbitrarySized n := returnGen (get_fresh_atoms n []) |}.
+Definition gen_id := gen_fresh id_store.
 
 Instance shrink_id : Shrink id := {| shrink x := [] |}.
 
 Instance show_id: Show id :=
   {| show x :=
-       ("Id "%string ++ (show x) ++ "")%string |}.
+       ("Id "%string ++ (show (Atom.nat_of x)) ++ "")%string |}.
 
 (* Sample (@arbitrary id _). *)
 
@@ -41,8 +38,8 @@ Instance show_aexp: Show aexp :=
   {| show := (
        fix show_aexp_func a :=
            match a with
-           | ANum n => "ANum " ++ (show n)
-           | AId ident => show ident
+           | ANum n => "ANum " ++ (show_nat n)
+           | AId ident => "Id " ++ show_nat (Atom.nat_of ident)
            | APlus a1 a2 => "(" ++ (show_aexp_func a1) ++ " + " ++
                                (show_aexp_func a2) ++ ")"
            | AMinus a1 a2 => "(" ++ (show_aexp_func a1) ++ " - " ++
@@ -52,10 +49,11 @@ Instance show_aexp: Show aexp :=
            end)%string
   |}.
 
+Derive Arbitrary for aexp.
+
 (** ** bexp **)
 
 Derive Show for bexp.
-
 
 Instance show_bexp: Show bexp :=
   {| show :=
@@ -70,22 +68,7 @@ Instance show_bexp: Show bexp :=
          end)%string
   |}.
 
-(*
-Instance gen_bexp_with_small_aexp `{GenSized aexp} : GenSized bexp :=
-  {| arbitrarySized :=
-       fix gen_bexp_func n :=
-         match n with
-         | 0 => elems [BTrue ; BFalse]
-         | S n' =>
-           let beq_gen := liftGen2 BEq (arbitrarySized 1) (arbitrarySized 1) in
-           let ble_gen := liftGen2 BLe (arbitrarySized 1) (arbitrarySized 1) in
-           let bnot_gen := liftGen BNot (gen_bexp_func n') in
-           let band_gen := liftGen2 BAnd (gen_bexp_func n') (gen_bexp_func n')
-           in
-           oneOf [ beq_gen ; ble_gen ; bnot_gen ; band_gen ]
-         end
-  |}.
-*)
+Derive Arbitrary for bexp.
 
 (** ** com **)
 
@@ -94,82 +77,17 @@ Instance show_com `{Show aexp} `{Show bexp} : Show com :=
   {| show :=
        fix show_com_func c := (
          match c with
-         | CSkip => "Skip"
-         | x ::= a => show_nat (Atom.nat_of x) ++ " := " ++ (show a)
-         | CSeq c1 c2 => (show_com_func c1) ++ ";" ++ newline ++ (show_com_func c2)
-         | CIf b c1 c2 => "If (" ++ (show b) ++ ") then "
-                                ++ (show_com_func c1) ++ " else "
-                                ++ (show_com_func c2) ++ " endIf"
-         | CWhile b c => "While (" ++ (show b) ++ ") do "
-                                  ++ (show_com_func c) ++ " endWhile"
+         | CSkip => "SKIP"
+         | x ::= a => "Id " ++ show_nat (Atom.nat_of x) ++ " := " ++ (show a)
+         | CSeq c1 c2 =>
+           (show_com_func c1) ++ "; " ++ (show_com_func c2)
+         | CIf b c1 c2 => "IFB " ++ (show b) ++ " THEN "
+                                ++ (show_com_func c1) ++ " ELSE "
+                                ++ (show_com_func c2) ++ " FI "
+         | CWhile b c => "WHILE " ++ (show b) ++ " DO "
+                                  ++ (show_com_func c) ++ " END"
          end)%string
   |}.
 
-(*
-Instance gen_seq_and_assgn_com `{Gen id} `{Gen aexp} `{Gen bexp} : GenSized com :=
-  {| arbitrarySized :=
-       fix com_gen_func n :=
-         match n with
-         | 0 => liftGen2 CAss arbitrary arbitrary
-         | S n' =>
-           let gen := com_gen_func n' in
-           liftGen2 CSeq gen gen
-         end
-  |}.
-*)
-
-(*
-Instance gen_if_com `{Gen id} `{Gen aexp} `{Gen bexp} : GenSized com :=
-  {| arbitrarySized :=
-       fix com_gen_func n :=
-         match n with
-         | 0 => freq [(2, returnGen CSkip) ;
-                       (6, liftGen2 CAss arbitrary arbitrary)]
-         | S n' =>
-           let gen := com_gen_func n' in
-           oneOf [liftGen3 CIf arbitrary gen gen; liftGen2 CSeq gen gen]
-         end
-  |}.
- *)
-
-(** EX: Write a generator that generates only IF-THEN-ELSE ... *)
-
-(* Sample (@arbitrarySized com gen_if_com 2). *)
-
-(** ** imp_state **)
-
-Record imp_state : Type := mk_imp_state { imp_st: state; imp_dom: list Atom.t }.
-
-Definition gen_state_from_atom_list
-           `{Gen nat}
-           (atom_list : list Atom.t) : G state :=
-  bindGen (vectorOf (List.length atom_list) arbitrary) (fun nat_list => 
-  returnGen (fun (a : Atom.t) =>
-               match (index_of_atom_in_list a atom_list) with
-               | None => 0
-               | Some i =>
-                 List.nth i nat_list 0
-               end)).
- 
-Instance gen_imp_state : GenSized imp_state :=
-  {| arbitrarySized n :=
-       let mem_dom := get_fresh_atoms n [] in
-       let gmem := gen_state_from_atom_list mem_dom in
-       bindGen gmem (fun mem =>
-         returnGen (mk_imp_state mem mem_dom))
-  |}.
-
-Definition show_image_given_domain `{Show A}
-           (f: Atom.t -> A) (l: list Atom.t) 
-           (prefix: string) : string := 
-  ((List.fold_left
-      (fun accum atom =>
-         accum ++ "(" ++ prefix ++ " " ++ (show atom) ++ ", "
-               ++ show (f atom) ++ ") ")
-      l "[") ++ "]")%string.
-                   
-Instance show_imp_state: Show imp_state :=
-  {| show x :=
-     "imp_state: " ++ (show_image_given_domain (imp_st x)
-                                               (imp_dom x) "")
-  |}.
+Remove Hints genSaexp : typeclass_instances.
+Remove Hints genSbexp : typeclass_instances.
