vminus/OpSemGen.v
@@ -10,6 +10,8 @@ Require Import String.
 Require Import QuickChick.QuickChick.
 Import QcDefaultNotation. Open Scope qc_scope.
 
+Require Import Vminus.QC.
+
 Require Import Vminus.Atom.
 Require Import Vminus.Vminus.
 Require Import Vminus.CFG.
@@ -33,101 +35,40 @@ Definition show_image_given_domain `{Show A}
       l "[") ++ "]")%string.
                    
 (** Opsem **)
+Definition locals_store := get_fresh_atoms 10 [].
 
-Definition show_memory
+Definition show_memory_on_domain
            (mem: mem) (dom: list Atom.t) : string :=
   "mem: " ++ (show_image_given_domain mem dom "addr").
 
-Definition show_locals
+Definition show_locals_on_domain
            (loc: loc) (dom: list Atom.t): string :=
   "locals: " ++ (show_image_given_domain loc dom "uid").
 
+Definition show_locals
+           (loc: loc): string := show_locals_on_domain loc locals_store.
 
-(*
-Record vminus_state : Type :=
-  mk_vminus_state {
-    vst_mem: mem;
-    vst_mem_dom: list Atom.t;
-    vst_pc: pc;
-    vst_loc: loc;
-    vst_loc_dom: list Atom.t;
-    vst_ppc: pc;
-    vst_ploc: loc;
-    vst_ploc_dom: list Atom.t
-  }.
-*)
-
-Definition gen_loc_from_atom_list
+Definition gen_loc_with_domain
            (atom_list : list Atom.t) : G loc :=
-  bindGen (vectorOf (List.length atom_list) arbitrary) (fun nat_list => 
-  returnGen (fun (a : Atom.t) =>
-               match (index_of_atom_in_list a atom_list) with
-               | None => None
-               | Some i =>
-                 List.nth_error nat_list i
-               end)).
+  nat_list <- vectorOf (List.length atom_list) arbitrary ;;
+  ret (fun (a : Atom.t) =>
+         match (index_of_atom_in_list a atom_list) with
+         | None => None
+         | Some i =>
+           List.nth_error nat_list i
+         end).
 
-Definition gen_mem_from_atom_list
+Definition gen_loc := gen_loc_with_domain locals_store.
+
+Definition gen_mem_with_domain
            (atom_list : list Atom.t) : G mem :=
-  bindGen (vectorOf (List.length atom_list) arbitrary) (fun nat_list => 
-  returnGen (fun (a : Atom.t) =>
-               match (index_of_atom_in_list a atom_list) with
-               | None => 0
-               | Some i =>
-                 List.nth i nat_list 0
-               end)).
-
-(*
-Definition gen_opsem_vminus_state: GenSized vminus_state :=
-  {| arbitrarySized n :=
-       let mem_dom := get_fresh_atoms n [] in
-       let loc_dom := get_fresh_atoms n [] in
-       let gmem := gen_mem_from_atom_list mem_dom in
-       let gloc := gen_loc_from_atom_list mem_dom in
-
-       bindGen gmem (fun mem =>
-       bindGen arbitrary (fun pc =>
-       bindGen gloc (fun loc =>
-       bindGen arbitrary (fun ppc =>
-       bindGen gloc (fun prev_loc =>
-         returnGen
-           (mk_vminus_state mem mem_dom
-                            pc
-                            loc loc_dom
-                            ppc
-                            prev_loc loc_dom))))))
-  |}.
-
-Instance show_vminus_state `{Show pc} : Show vminus_state :=
-  {| show st :=
-       let 'mk_vminus_state mem mem_dom
-                            pc
-                            loc loc_dom
-                            ppc
-                            prev_loc prev_loc_dom := st in
-       (show_memory mem mem_dom ++ ", " ++
-        "pc: " ++ show pc ++ ", " ++
-        show_locals loc loc_dom ++ ", " ++
-        "ppc: " ++ show ppc ++ ", " ++
-        "prev_loc: " ++
-        show_locals prev_loc prev_loc_dom)%string
-  |}.
-
-Definition vst_to_state (vst: vminus_state) :=
-  mkst (vst_mem vst) (vst_pc vst) (vst_loc vst)
-               (vst_ppc vst) (vst_ploc vst).
-*)
-
-(*
-Fixpoint generate_dummy_insns (n : nat) : list insn :=
-  let fixed_addr := Atom.fresh [] in
-  let fixed_uid := Atom.fresh [] in
-  match n with
-  | 0 => []
-  | S n' =>
-    (fixed_uid, cmd_load fixed_addr) :: generate_dummy_insns n'
-  end.
- *)
+  nat_list <- vectorOf (List.length atom_list) arbitrary ;;
+  ret (fun (a : Atom.t) =>
+         match (index_of_atom_in_list a atom_list) with
+         | None => 0
+         | Some i =>
+           List.nth i nat_list 0
+         end).
 
 Definition generate_dummy_insns n: list insn :=
   let atoms := (get_fresh_atoms n []) in
@@ -140,7 +81,6 @@ Definition generate_dummy_insns n: list insn :=
       end
   in List.rev (helper n).
 
-(* TODO: proper generator *)
 (* Returns a CFG with a single block containing instrs ++ instrs_after, 
     and the pc in that block that begins at instrs_after *)
 Definition wrap_code_in_cfg (p: pc) (instrs instrs_after: list insn)
